James C - cleaned up 8, 9, 10, 11

isabelle/Chapter08_1_Language.thy
@@ -31,37 +31,16 @@ where "insert n (Var v) = Var (incr n v)"
     | "insert n (Lam t e) = Lam t (insert (next n) e)"
     | "insert n (Appl e1 e2) = Appl (insert n e1) (insert n e2)"
 
-primrec remove :: "var => expr => expr"
-where "remove n (Var v) = Var (subr n v)"
-    | "remove n (Num x) = Num x"
-    | "remove n (Str s) = Str s"
-    | "remove n (Plus e1 e2) = Plus (remove n e1) (remove n e2)"
-    | "remove n (Times e1 e2) = Times (remove n e1) (remove n e2)"
-    | "remove n (Cat e1 e2) = Cat (remove n e1) (remove n e2)"
-    | "remove n (Len e) = Len (remove n e)"
-    | "remove n (Let e1 e2) = Let (remove n e1) (remove (next n) e2)"
-    | "remove n (Lam t e) = Lam t (remove (next n) e)"
-    | "remove n (Appl e1 e2) = Appl (remove n e1) (remove n e2)"
-
-primrec subst' :: "var => expr => expr => expr"
-where "subst' n e' (Var v) = (if v = n then e' else Var v)"
-    | "subst' n e' (Num x) = Num x"
-    | "subst' n e' (Str s) = Str s"
-    | "subst' n e' (Plus e1 e2) = Plus (subst' n e' e1) (subst' n e' e2)"
-    | "subst' n e' (Times e1 e2) = Times (subst' n e' e1) (subst' n e' e2)"
-    | "subst' n e' (Cat e1 e2) = Cat (subst' n e' e1) (subst' n e' e2)"
-    | "subst' n e' (Len e) = Len (subst' n e' e)"
-    | "subst' n e' (Let e1 e2) = Let (subst' n e' e1) (subst' (next n) (insert first e') e2)"
-    | "subst' n e' (Lam t e) = Lam t (subst' (next n) (insert first e') e)"
-    | "subst' n e' (Appl e1 e2) = Appl (subst' n e' e1) (subst' n e' e2)"
-
-definition subst :: "expr => var => expr => expr"
-where "subst e' n e = remove first (subst' first (insert first e') e)"
-
-lemma [simp]: "remove n (insert n e) = e"
-by (induction e arbitrary: n, simp_all)
-
-lemma [simp]: "canswap m n ==> insert m (insert n e) = insert (next n) (insert m e)"
-by (induction e arbitrary: n m, simp_all)
+primrec subst :: "expr => var => expr => expr"
+where "subst e' n (Var x) = (if x = n then e' else Var (subr n x))"
+    | "subst e' n (Num x) = Num x"
+    | "subst e' n (Str s) = Str s"
+    | "subst e' n (Plus e1 e2) = Plus (subst e' n e1) (subst e' n e2)"
+    | "subst e' n (Times e1 e2) = Times (subst e' n e1) (subst e' n e2)"
+    | "subst e' n (Cat e1 e2) = Cat (subst e' n e1) (subst e' n e2)"
+    | "subst e' n (Len e) = Len (subst e' n e)"
+    | "subst e' n (Let e1 e2) = Let (subst e' n e1) (subst (insert first e') (next n) e2)"
+    | "subst e' n (Lam t e) = Lam t (subst (insert first e') (next n) e)"
+    | "subst e' n (Appl e1 e2) = Appl (subst e' n e1) (subst e' n e2)"
 
 end
